simplifications + renamings

tarjan_nocolors.v
@@ -17,8 +17,8 @@ Notation infty := #|V|.+1.
 
 Record env := Env {esccs : {set {set V}}; num: {ffun V -> nat}}.
 
-Definition seen e := [set x | num e x < infty].
-Notation sn e := #|seen e|.
+Definition visited e := [set x | num e x < infty].
+Notation sn e := #|visited e|.
 Definition stack e := [set x | num e x < sn e].
 Notation new_stack e1 e2 := (stack e2 :\: stack e1).
 
@@ -147,26 +147,26 @@ Qed.
 (* Well formed env *)
 (*******************)
 
-Lemma num_lt_infty e x : num e x < infty = (x \in seen e).
+Lemma num_lt_infty e x : num e x < infty = (x \in visited e).
 Proof. by rewrite inE. Qed.
 
 Lemma num_lt_sn e x : num e x < sn e = (x \in stack e).
 Proof. by rewrite inE. Qed.
 
-Lemma seen_visit e x : seen (visit x e) = x |: seen e.
+Lemma visited_visit e x : visited (visit x e) = x |: visited e.
 Proof.
 apply/setP=> y; rewrite !inE ffunE/=; case: (altP eqP);
 by rewrite //= ltnS max_card.
 Qed.
 
-Lemma sub_stack_seen e : stack e \subset seen e.
+Lemma sub_stack_visited e : stack e \subset visited e.
 Proof.
 apply/subsetP => x; rewrite !inE => /leq_trans; apply;
 by rewrite leqW// max_card.
 Qed.
 
-Lemma sub_new_stack_seen e1 e2: new_stack e1 e2 \subset seen e2.
-Proof. by rewrite (subset_trans _ (sub_stack_seen _)) ?subsetDl. Qed.
+Lemma sub_new_stack_visited e1 e2: new_stack e1 e2 \subset visited e2.
+Proof. by rewrite (subset_trans _ (sub_stack_visited _)) ?subsetDl. Qed.
 
 Section wfenv.
 
@@ -180,7 +180,7 @@ Record wf_env e := WfEnv {
 
 Variables (e : env) (e_wf : wf_env e).
 
-Lemma notseen_num x : x \notin seen e -> num e x = infty.
+Lemma notvisited_num x : x \notin visited e -> num e x = infty.
 Proof. by rewrite inE ltn_neqAle max_num// andbT negbK => /eqP. Qed.
 
 Lemma num_lt_V x : (num e x < #|V|) = (num e x < sn e).
@@ -189,7 +189,7 @@ apply/idP/idP => [/num_lt_V_is_stack//|]; first exact.
 by move=> /leq_trans; apply; rewrite max_card.
 Qed.
 
-Lemma num_lt_card x (A : pred V) : seen e \subset A ->
+Lemma num_lt_card x (A : pred V) : visited e \subset A ->
   (num e x < #|A|) = (num e x < sn e).
 Proof.
 move=> subeA; apply/idP/idP => /leq_trans.
@@ -197,7 +197,7 @@ move=> subeA; apply/idP/idP => /leq_trans.
 by apply; rewrite subset_leq_card.
 Qed.
 
-Lemma seenE : seen e = stack e :|: cover (esccs e).
+Lemma visitedE : visited e = stack e :|: cover (esccs e).
 Proof.
 by apply/setP=> x; rewrite !inE ltnS leq_eqVlt -num_sccs// num_lt_V orbC.
 Qed.
@@ -208,13 +208,13 @@ rewrite -setI_eq0; apply/eqP/setP=> x; rewrite !inE -num_sccs//.
 by rewrite -num_lt_V; case: ltngtP.
 Qed.
 
-Lemma sub_sccs_seen : cover (esccs e) \subset seen e.
+Lemma sub_sccs_visited : cover (esccs e) \subset visited e.
 Proof. by apply/subsetP => x; rewrite !inE -num_sccs// => /eqP->. Qed.
 
-Lemma stack_visit x : x \notin seen e -> stack (visit x e) = x |: stack e.
+Lemma stack_visit x : x \notin visited e -> stack (visit x e) = x |: stack e.
 Proof.
-move=> xNseen; apply/setP=> y; rewrite !inE/= ffunE/= seen_visit.
-have [->|neq_yx]//= := altP eqP; first by rewrite cardsU1 xNseen ltnS ?leqnn.
+move=> xNvisited; apply/setP=> y; rewrite !inE/= ffunE/= visited_visit.
+have [->|neq_yx]//= := altP eqP; first by rewrite cardsU1 xNvisited ltnS ?leqnn.
 by rewrite num_lt_card// subsetUr.
 Qed.
 
@@ -222,19 +222,19 @@ End wfenv.
 
 Lemma wf_visit e x : wf_env e ->
    (forall y, num e y < sn e -> gconnect y x) ->
-   x \notin seen e -> wf_env (visit x e).
+   x \notin visited e -> wf_env (visit x e).
 Proof.
-move=> e_wf x_connected xNseen; constructor=> [|y|y|y|] //=; rewrite ?inE ?ffunE/=.
+move=> e_wf x_connected xNvisited; constructor=> [|y|y|y|] //=; rewrite ?inE ?ffunE/=.
 - exact: sub_gsccs.
 - by case: ifP; rewrite ?max_num// leqW ?max_card.
-- rewrite seen_visit cardsU1 xNseen; case: ifPn => // _.
+- rewrite visited_visit cardsU1 xNvisited; case: ifPn => // _.
   by rewrite num_lt_V// ltnS => /ltnW.
 - have [->|] := altP (y =P x); last by rewrite num_sccs.
-  rewrite -num_sccs// notseen_num// eq_sym !gtn_eqF//.
-  by rewrite (@leq_trans #|x |: seen e|) ?max_card// cardsU1 xNseen.
+  rewrite -num_sccs// notvisited_num// eq_sym !gtn_eqF//.
+  by rewrite (@leq_trans #|x |: visited e|) ?max_card// cardsU1 xNvisited.
 move=> y z; rewrite !ffunE/=.
-have sub_visit : seen e \subset seen (visit x e).
-  by apply/subsetP => ?; rewrite seen_visit !inE orbC => ->.
+have sub_visit : visited e \subset visited (visit x e).
+  by apply/subsetP => ?; rewrite visited_visit !inE orbC => ->.
 have [{y}->|neq_yx] := altP eqP; have [{z}->|neq_zx]//= := altP eqP.
 + by rewrite num_lt_card//; case: ltngtP.
 + move=> /andP[/leq_ltn_trans lt/lt].
@@ -267,14 +267,14 @@ have nume1_lt := num_lt x; apply/idP/idP => // {nume1_lt}nume1_lt.
 by rewrite num_eq ?inE// (leq_trans nume1_lt)// leqW// max_card.
 Qed.
 
-Lemma sub_seen e1 e2 : subenv e1 e2 -> seen e1 \subset seen e2.
+Lemma sub_visited e1 e2 : subenv e1 e2 -> visited e1 \subset visited e2.
 Proof.
-move=> sube12; apply/subsetP=> x; rewrite !inE => x_seen1.
+move=> sube12; apply/subsetP=> x; rewrite !inE => x_visited1.
 by rewrite (sub_snum sube12)// inE.
 Qed.
 
 Lemma leq_sn e1 e2 : subenv e1 e2 -> sn e1 <= sn e2.
-Proof. by move=> sube12; rewrite subset_leq_card// sub_seen. Qed.
+Proof. by move=> sube12; rewrite subset_leq_card// sub_visited. Qed.
 
 Lemma sub_stack e1 e2 : subenv e1 e2 -> stack e1 \subset stack e2.
 Proof.
@@ -292,20 +292,20 @@ have [e1_after|e1_before] /= := leqP (sn e1) (num e1 x).
 by rewrite leqNgt -sub_num_lt// e1_before.
 Qed.
 
-Notation new_seen e1 e2 := (seen e2 :\: seen e1).
+Notation new_visited e1 e2 := (visited e2 :\: visited e1).
 
-Lemma new_seenE e1 e2 : wf_env e1 -> wf_env e2 -> subenv e1 e2 ->
-(new_seen e1 e2) = (new_stack e1 e2) :|: cover (esccs e2) :\: cover (esccs e1).
+Lemma new_visitedE e1 e2 : wf_env e1 -> wf_env e2 -> subenv e1 e2 ->
+(new_visited e1 e2) = (new_stack e1 e2) :|: cover (esccs e2) :\: cover (esccs e1).
 Proof.
-move=> e1_wf e2_wf sube12; rewrite !seenE//; apply/setP=> x.
+move=> e1_wf e2_wf sube12; rewrite !visitedE//; apply/setP=> x.
 rewrite !inE -!num_sccs -?num_lt_V//; do 2!case: ltngtP => //=.
   by rewrite num_lt_V// (sub_num_lt sube12)// => ->; rewrite ltnNge max_card.
 by move=> xe2 xe1; move: xe2; rewrite (sub_snum sube12)// ?xe1// ltnn.
 Qed.
 
-Lemma sub_new_stack_new_seen e1 e2 : subenv e1 e2 -> wf_env e1 -> wf_env e2 ->
-  (new_stack e1 e2) \subset (new_seen e1 e2).
-Proof. by move=> e1_wf e2_wf sube12; rewrite (@new_seenE e1 e2)// subsetUl. Qed.
+Lemma sub_new_stack_new_visited e1 e2 : subenv e1 e2 -> wf_env e1 -> wf_env e2 ->
+  (new_stack e1 e2) \subset (new_visited e1 e2).
+Proof. by move=> e1_wf e2_wf sube12; rewrite (@new_visitedE e1 e2)// subsetUl. Qed.
 
 Lemma sub_refl e : subenv e e.
 Proof. by rewrite /subenv !subxx /=; apply/andP; split; apply/forall_inP. Qed.
@@ -321,30 +321,24 @@ have x2 : num e3 x < sn e2 by rewrite (leq_trans xP)// leq_sn.
 by rewrite (sub_num_lt sub12)// -(sub_vnum sub23)// (sub_num_lt sub23).
 Qed.
 
-Lemma sub_visit e x : x \notin seen e -> subenv e (visit x e).
+Lemma sub_visit e x : x \notin visited e -> subenv e (visit x e).
 Proof.
-move=> xNseen; rewrite /subenv subxx/=; apply/andP; split; last first.
+move=> xNvisited; rewrite /subenv subxx/=; apply/andP; split; last first.
   by apply/forall_inP => y; rewrite !ffunE/=; case: ifP; rewrite ?ltnn.
 apply/forall_inP => y y_in; rewrite !ffunE/=.
-by case: (altP (y =P x)) xNseen => // <-; rewrite inE y_in.
+by case: (altP (y =P x)) xNvisited => // <-; rewrite inE y_in.
 Qed.
 
-Lemma stackE e : wf_env e -> stack e = seen e :\: cover (esccs e).
-Proof.
-move=> e_wf; apply/setP=> x; rewrite seenE// setDUl setDv setU0.
-by rewrite !inE -num_sccs// -num_lt_V//; case: ltngtP.
-Qed.
-
-Lemma seen_store (A : {set V}) e : A \subset seen e -> seen (store A e) = seen e.
+Lemma visited_store (A : {set V}) e : A \subset visited e -> visited (store A e) = visited e.
 Proof.
 move=> A_sub; apply/setP=> x; rewrite !inE/= ffunE.
 by case: ifPn => // /(subsetP A_sub); rewrite inE leqnn => ->.
 Qed.
 
-Lemma stack_store (A : {set V}) e : A \subset seen e ->
+Lemma stack_store (A : {set V}) e : A \subset visited e ->
   stack (store A e) = stack e :\: A.
 Proof.
-move=> A_sub; apply/setP => x; rewrite !inE seen_store//= ffunE.
+move=> A_sub; apply/setP => x; rewrite !inE visited_store//= ffunE.
 by case: (x \in A); rewrite //= ltnNge max_card.
 Qed.
 
@@ -355,19 +349,19 @@ Qed.
 Definition outenv (roots : {set V}) (e e' : env) := [/\
   {in new_stack e e' &, gconnected},
   {in new_stack e e', forall x, exists2 y, y \in stack e & gconnect x y} &
-  seen e' = seen e :|: nexts (~: seen e) roots ].
+  visited e' = visited e :|: nexts (~: visited e) roots ].
 
 Variant dfs_spec_def (dfs : nat * env) (roots : {set V}) e :
   (nat * env) -> nat -> env -> Type := DfsSpec me' m e' of
     me' = (m, e') &
-    m = val (\min_(x in nexts (~:seen e) roots) @inord #|V| (num e' x)) &
+    m = val (\min_(x in nexts (~:visited e) roots) @inord #|V| (num e' x)) &
     wf_env e' & subenv e e' & outenv roots e e' :
   dfs_spec_def dfs roots e me' m e'.
 Notation dfs_spec dfs roots e := (dfs_spec_def dfs roots e dfs dfs.1 dfs.2).
 
 Definition dfs_correct dfs (roots : {set V}) e := wf_env e ->
   {in stack e & roots, gconnected} -> dfs_spec (dfs roots e) roots e.
-Definition dfs1_correct dfs1 x e := wf_env e -> x \notin seen e ->
+Definition dfs1_correct dfs1 x e := wf_env e -> x \notin visited e ->
   {in stack e & [set x], gconnected} -> dfs_spec (dfs1 x e) [set x] e.
 
 (*****************)
@@ -388,30 +382,30 @@ case: pickP => /= [x x_roots|]; last first.
     by move=> ?; rewrite inE.
 have [numx_infty|numx_ninfty]/= := altP eqP; last first.
   have numx_lt : num e x < infty by rewrite ltn_neqAle numx_ninfty max_num.
-  have x_seen : x \in seen e by rewrite inE.
-  case: dfsP => //= [u v ve|_ _ e1 -> -> e1_wf subee1 [new1c new1old seen1E]].
+  have x_visited : x \in visited e by rewrite inE.
+  case: dfsP => //= [u v ve|_ _ e1 -> -> e1_wf subee1 [new1c new1old visited1E]].
     by rewrite inE => /andP[_ v_roots]; rewrite roots_connected.
   constructor => //=.
-    rewrite -[in RHS](setD1K x_roots) nextsU nexts1 inE x_seen/= setU0.
+    rewrite -[in RHS](setD1K x_roots) nextsU nexts1 inE x_visited/= setU0.
     by rewrite bigmin_setU /= big_set1/= (@sub_snum e e1)// inordK//.
-  constructor=> //=; rewrite -(setD1K x_roots) nextsU nexts1 inE x_seen/=.
+  constructor=> //=; rewrite -(setD1K x_roots) nextsU nexts1 inE x_visited/=.
   by rewrite setU0 setUCA setUA [x |: _](setUidPr _) ?sub1set.
 case: dfs1P => //=; first by rewrite inE numx_infty ltnn.
   by move=> u v ue; rewrite inE => /eqP->; apply: roots_connected.
-move=> _ _  e1 -> -> e1_wf subee1 [new1c new1old seen1E].
-case: dfsP => //= [u v ue1|_ _ e2 -> -> e2_wf sube12 [new2c new2old seen2E]].
+move=> _ _  e1 -> -> e1_wf subee1 [new1c new1old visited1E].
+case: dfsP => //= [u v ue1|_ _ e2 -> -> e2_wf sube12 [new2c new2old visited2E]].
   rewrite inE => /andP[_ v_roots].
   have [ue|uNe] := boolP (u \in stack e); first by rewrite roots_connected.
   have [|w we] := new1old u; first by rewrite inE ue1 uNe.
   by move=> /connect_trans->//; rewrite roots_connected//.
 have sube2 : subenv e e2 by exact: sub_trans sube12.
-have nexts_split : nexts (~: seen e) roots =
-      nexts (~: seen e) [set x] :|: nexts (~: seen e1) (roots :\ x).
-  by rewrite -[in LHS](setD1K x_roots) nextsU seen1E setCU nextsUI// nexts_id.
+have nexts_split : nexts (~: visited e) roots =
+      nexts (~: visited e) [set x] :|: nexts (~: visited e1) (roots :\ x).
+  by rewrite -[in LHS](setD1K x_roots) nextsU visited1E setCU nextsUI// nexts_id.
 constructor => //=.
   rewrite (eq_bigr (fun x => inord (num e2 x))); last first.
     move=> y y_in; rewrite (@sub_snum e1 e2)// num_lt_infty.
-      by rewrite seen1E setUC inE y_in.
+      by rewrite visited1E setUC inE y_in.
   by rewrite -[LHS]/(val (ord_minn _ _)) -bigmin_setU /= -nexts_split.
 constructor => /=.
 + rewrite -(@setUD _ (stack e1)) ?sub_stack//.
@@ -433,40 +427,40 @@ constructor => /=.
     by exists r; rewrite ?inE.
   have [|r' r's rr'] := new1old r; first by rewrite ?inE -leqNgt r_ge r_lt1.
   by exists r'; rewrite // (connect_trans yr rr').
-+ by rewrite seen2E {1}seen1E nexts_split setUA.
++ by rewrite visited2E {1}visited1E nexts_split setUA.
 Qed.
 
 Lemma dfs1P dfs x e (A := [set y in successors x]):
   dfs_correct dfs A (visit x e) -> dfs1_correct (dfs1 dfs) x e.
 Proof.
-rewrite /dfs1 => dfsP e_wf xNseen x_connected.
+rewrite /dfs1 => dfsP e_wf xNvisited x_connected.
 have subexe: subenv e (visit x e) by exact: sub_visit.
-have num0x : num e x = infty by apply: notseen_num.
+have num0x : num e x = infty by apply: notvisited_num.
 have xNstack : x \notin stack e.
   by rewrite inE num0x ltnNge leqW// max_card.
 have xe_wf : wf_env (visit x e).
   by apply: wf_visit => // y y_lt; rewrite x_connected ?inE.
-have nexts1E : nexts (~: seen e) [set x] = x |: nexts (~: (x |: seen e)) A.
+have nexts1E : nexts (~: visited e) [set x] = x |: nexts (~: (x |: visited e)) A.
   by rewrite nexts1_split ?setDE ?setCU 1?setIC 1?inE.
 case: dfsP => //=.
   rewrite stack_visit// => u v; rewrite in_setU1=> /predU1P[->|ue];
   rewrite inE => /(@connect1 _ edge)// /(connect_trans _)->//.
   by rewrite x_connected// set11.
-move=> _ _ e1 //= -> -> e1_wf subxe1 [newc new_old seen1E].
+move=> _ _ e1 //= -> -> e1_wf subxe1 [newc new_old visited1E].
 have sube1 : subenv e e1 by apply: sub_trans subxe1.
 have num1x : num e1 x = sn e.
   by rewrite (sub_snum subxe1)// ?inE ?ffunE/= ?eqxx// ltnS max_card.
-rewrite seen_visit in seen1E *.
+rewrite visited_visit in visited1E *.
 have lt_sn_sn1 : sn e < sn e1.
-  by rewrite (leq_trans _ (leq_sn subxe1))// seen_visit cardsU1 xNseen.
-have x_seen1 : x \in seen e1 by rewrite seen1E inE setU11.
+  by rewrite (leq_trans _ (leq_sn subxe1))// visited_visit cardsU1 xNvisited.
+have x_visited1 : x \in visited e1 by rewrite visited1E inE setU11.
 have x_stack : x \in stack e1.
   by rewrite (subsetP (sub_stack subxe1))//= stack_visit// setU11.
 have [min_after|min_before] := leqP; last first.
   constructor => //=.
     rewrite nexts1E bigmin_setU big_set1 /= inordK ?num1x ?ltnS ?max_card//.
     by rewrite (minn_idPr _)// ltnW.
-  constructor=> //=; last by rewrite nexts1E setUCA setUA seen1E.
+  constructor=> //=; last by rewrite nexts1E setUCA setUA visited1E.
     move=> y z; have [-> _|neq_yx] := eqVneq y x.
       by rewrite new_stackE ?inE// -num1x; apply: le_connect.
     rewrite -(@setUD _ (stack (visit x e))) ?sub_stack//.
@@ -476,14 +470,14 @@ have [min_after|min_before] := leqP; last first.
     move=> y_e1 /predU1P[->|]; last exact: newc y_e1.
     have [t] := new_old y y_e1; rewrite !inE => t_le /connect_trans->//.
     rewrite (@le_connect (visit x e))// andbC; move: t_le.
-    by rewrite seen_visit !ffunE /= eqxx cardsU1 xNseen add1n !ltnS leqnn.
+    by rewrite visited_visit !ffunE /= eqxx cardsU1 xNvisited add1n !ltnS leqnn.
   move=> y; have [v ve xv] : exists2 v, v \in stack e & gconnect x v.
-    have [|v] := @eq_bigmin_cond _ _ (mem (nexts (~: (x |: seen e)) A))
+    have [|v] := @eq_bigmin_cond _ _ (mem (nexts (~: (x |: visited e)) A))
                                (@inord #|V| \o (num e1)).
       rewrite card_gt0; apply: contraTneq min_before => ->.
       by rewrite big_set0 -leqNgt max_card.
     rewrite !inE => v_in min_is_v; move: min_before; rewrite min_is_v/=.
-    rewrite inordK; last by rewrite num_lt_infty seen1E inE v_in orbT.
+    rewrite inordK; last by rewrite num_lt_infty visited1E inE v_in orbT.
     rewrite -sub_num_lt// => v_lt; exists v; rewrite ?inE//.
     move: v_in => /in_nextsW[z]; rewrite inE => /(@connect1 _ edge).
     by apply: connect_trans.
@@ -494,23 +488,23 @@ have [min_after|min_before] := leqP; last first.
   move=> /new_old[z]; rewrite stack_visit// in_setU1.
   move=> /predU1P[->|]; last by exists z.
   by move=> yx; exists v; rewrite // (connect_trans yx).
-have all_geq y : y \in nexts (~: seen e) [set x] ->
-  (#|seen e| <= num e1 y) * (num e1 y < infty).
+have all_geq y : y \in nexts (~: visited e) [set x] ->
+  (#|visited e| <= num e1 y) * (num e1 y < infty).
   have := min_after; have sn_inord : sn e = @inord #|V| (sn e).
     by rewrite inordK// ltnS max_card.
   rewrite {1}sn_inord; move/bigmin_geqP => /(_ y) y_ge.
   rewrite nexts1E !inE => /predU1P[->|yA]; rewrite ?num1x.
     by rewrite ltnS max_card leqnn.
   rewrite sn_inord (leq_trans (y_ge _))// ?inordK//;
-  by rewrite num_lt_infty seen1E 2!inE yA orbT.
+  by rewrite num_lt_infty visited1E 2!inE yA orbT.
 constructor => //=.
 - rewrite big1// => y xy; rewrite ffunE new_stackE ?inE//=.
-  have y_seen1 : num e1 y < infty.
-    by rewrite num_lt_infty seen1E -setUA setUCA -nexts1E inE xy orbT.
+  have y_visited1 : num e1 y < infty.
+    by rewrite num_lt_infty visited1E -setUA setUCA -nexts1E inE xy orbT.
   apply/val_inj=> /=; case: ifPn; rewrite ?inordK//.
-  rewrite all_geq//= -num_lt_V// -leqNgt; move: y_seen1; rewrite ltnS.
+  rewrite all_geq//= -num_lt_V// -leqNgt; move: y_visited1; rewrite ltnS.
   by case: ltngtP.
-- constructor => //=; rewrite ?seen_store ?sub_new_stack_seen//.
+- constructor => //=; rewrite ?visited_store ?sub_new_stack_visited//.
   + rewrite subUset sub_gsccs// andbT sub1set.
     suff -> : new_stack e e1 = gscc_of x by rewrite pblock_mem ?cover_sccs.
     apply/setP=> y; rewrite mem_scc /symconnect.
@@ -523,13 +517,13 @@ constructor => //=.
         have [z] := new_old _ y_xee1.
         rewrite stack_visit// in_setU1 => /predU1P[->//|/x_connected].
         by move=> /(_ _ (set11 x))/(connect_trans _) xz /xz.
-      have: y \in new_seen (visit x e) e1.
-        by apply: subsetP y_xee1; rewrite sub_new_stack_new_seen.
-      rewrite inE seen1E in_setU seen_visit//; case: (y \in _ |: _) => //=.
+      have: y \in new_visited (visit x e) e1.
+        by apply: subsetP y_xee1; rewrite sub_new_stack_new_visited.
+      rewrite inE visited1E in_setU visited_visit//; case: (y \in _ |: _) => //=.
       move=> /in_nextsW[z]; rewrite inE=> /(@connect1 _ edge).
       exact: connect_trans.
-    have /(connect_from (mem (~: seen e))) [z []] := xy; rewrite inE.
-    move=> eq_yz xz zy; have /all_geq [] : z \in nexts (~: seen e) [set x].
+    have /(connect_from (mem (~: visited e))) [z []] := xy; rewrite inE.
+    move=> eq_yz xz zy; have /all_geq [] : z \in nexts (~: visited e) [set x].
       by apply/bigcupP; exists x; rewrite !inE.
     rewrite leqNgt -sub_num_lt// -num_lt_V// -leqNgt ltnS => zNstack.
     have zNcover e' : wf_env e' -> z \in cover (esccs e') ->
@@ -541,16 +535,16 @@ constructor => //=.
     rewrite leq_eqVlt num_sccs// num_lt_V// => /orP[|z_stack].
        move=> /zNcover; rewrite -num_sccs// num1x => /(_ _) /eqP eq_V.
        by rewrite eq_V// ltnNge max_card in lt_sn_sn1.
-    have zNseen : z \notin seen e.
+    have zNvisited : z \notin visited e.
       rewrite inE -leqNgt ltn_neqAle eq_sym num_sccs// zNstack andbT.
       apply: contraTN isT => /(zNcover _ e_wf).
       by rewrite -num_sccs// num0x; elim: #|V|.
-    move: eq_yz; rewrite zNseen /= => /andP[/eqP eq_yz _].
+    move: eq_yz; rewrite zNvisited /= => /andP[/eqP eq_yz _].
     rewrite -eq_yz in zNstack z_stack.
     by rewrite !inE -num_lt_V// -leqNgt zNstack.
   + by move=> v; rewrite ffunE/=; case: ifP; rewrite ?max_num //.
   + move=> v; rewrite ffunE/=; case: ifPn; rewrite ?ltnn// => vNe12.
-    by rewrite num_lt_V// seen_store.
+    by rewrite num_lt_V// visited_store.
   + move=> v; rewrite ffunE /= cover1U [in RHS]inE.
     by case: ifPn; rewrite ?eqxx//= => vNe12; rewrite -num_sccs//.
   + move=> y z; rewrite !ffunE; case: ifPn => _.
@@ -562,14 +556,14 @@ constructor => //=.
     move=> vs; rewrite (sub_snum sube1)// leqNgt -!num_lt_V// -leqNgt ifN//.
     by apply/negP => /andP[/leq_ltn_trans Vlt/Vlt]; rewrite ltnNge max_card.
   by case: ifPn; [move=> _; rewrite ltnNge max_card|rewrite -sub_num_lt].
-- rewrite /outenv stack_store ?seen_store ?sub_new_stack_seen//.
+- rewrite /outenv stack_store ?visited_store ?sub_new_stack_visited//.
   rewrite setDDr setDUl setDv set0D set0U setDIl !setDv setI0.
   split; do ?by move=> ?; rewrite inE.
-  by rewrite seen1E -setUA setUCA -nexts1E.
+  by rewrite visited1E -setUA setUCA -nexts1E.
 Qed.
 
-Theorem tarjan_rec_terminates n (roots : {set V}) e :
-  n >= #|~: seen e| * #|V|.+1 + #|roots| ->
+Theorem tarjan_rec_term n (roots : {set V}) e :
+  n >= #|~: visited e| * #|V|.+1 + #|roots| ->
   dfs_correct (tarjan_rec n) roots e.
 Proof.
 move=> n_ge; elim: n => [|n IHn/=] in roots e n_ge *.
@@ -579,46 +573,39 @@ move=> n_ge; elim: n => [|n IHn/=] in roots e n_ge *.
 apply: dfsP=> x x_roots; last first.
   move=> e1 subee1; apply: IHn; rewrite -ltnS (leq_trans _ n_ge)//.
   rewrite (cardsD1 x roots) x_roots add1n -addSnnS ltn_add2r ltnS.
-  by rewrite leq_mul2r //= subset_leq_card// setCS sub_seen.
-move=> e_wf xNseen; apply: dfs1P => //; apply: IHn.
-rewrite seen_visit setCU setIC -setDE -ltnS (leq_trans _ n_ge)//.
-rewrite (cardsD1 x (~: _)) inE xNseen add1n mulSnr -addnA ltn_add2l.
+  by rewrite leq_mul2r //= subset_leq_card// setCS sub_visited.
+move=> e_wf xNvisited; apply: dfs1P => //; apply: IHn.
+rewrite visited_visit setCU setIC -setDE -ltnS (leq_trans _ n_ge)//.
+rewrite (cardsD1 x (~: _)) inE xNvisited add1n mulSnr -addnA ltn_add2l.
 by rewrite ltn_addr// ltnS max_card.
 Qed.
 
-Lemma seen0 : seen e0 = set0.
+Lemma visited0 : visited e0 = set0.
 Proof. by apply/setP=> y; rewrite !inE ffunE ltnn. Qed.
 
 Lemma stack0 : stack e0 = set0.
 Proof. by apply/setP=> y; rewrite !inE ffunE ltnNge leqW ?max_card. Qed.
 
-Lemma tarjan_recP : tarjan_rec N setT e0 = (#|V|, Env gsccs [ffun x => #|V|]).
+Theorem tarjan_correct : tarjan = gsccs.
 Proof.
-case: tarjan_rec_terminates; first by rewrite seen0 setC0 cardsT.
+rewrite /tarjan; case: tarjan_rec_term; first by rewrite visited0 setC0 cardsT.
 - constructor; rewrite /= ?sub0set// => x; rewrite !ffunE//.
   + by rewrite ltnNge leqW//.
   + by rewrite gtn_eqF// /cover big_set0 inE.
   + by move=> y; rewrite !ffunE//= andbC ltnNge leqW// ?max_card.
-  + by move=> y; rewrite !inE !ffunE/= ltnNge leqW// max_card.
-move=> _ _ e -> -> e_wf _ [_]; rewrite stack0 setD0.
+- by move=> y; rewrite !inE !ffunE/= ltnNge leqW// max_card.
+move=> _ _ e _ _ e_wf _ [_]; rewrite stack0 setD0.
 have [stacke _|[x xe]] := set_0Vmem (stack e); last first.
   by move=> /(_ _ xe)[?]; rewrite inE.
-rewrite seen0 set0U setC0 nextsT => seene.
+rewrite visited0 set0U setC0 nextsT => visitede.
 have numE x : num e x = #|V|.
-  apply/eqP; have /setP/(_ x) := seene.
-  by rewrite seenE// stacke set0U !inE -num_sccs.
-have sccse : esccs e = gsccs.
-  apply/eqP; rewrite eqEsubset sub_gsccs//=; apply/subsetP => _/imsetP[/=x _->].
-  have: x \in cover (esccs e) by rewrite -num_sccs ?numE//.
-  move=> /bigcupP [C Csccs /(def_scc (subsetP (sub_gsccs e_wf) _ Csccs))] eqC.
-  rewrite -eqC (_ : [set _ in _ | _] = gscc_of x)// in Csccs *.
-  by apply/setP => y; rewrite !inE mem_scc /=.
-rewrite big1; last by move=> x _; apply: val_inj; rewrite /= inordK// ?numE.
-congr (_, _); case: e {stacke seene e_wf} => /= sccs num in numE sccse *.
-by congr (Env _ _) => //; apply/ffunP=> x; rewrite ffunE.
+  apply/eqP; have /setP/(_ x) := visitede.
+  by rewrite visitedE// stacke set0U !inE -num_sccs.
+apply/eqP; rewrite eqEsubset sub_gsccs//=; apply/subsetP => _/imsetP[/=x _->].
+have: x \in cover (esccs e) by rewrite -num_sccs ?numE//.
+move=> /bigcupP [C Csccs /(def_scc (subsetP (sub_gsccs e_wf) _ Csccs))] eqC.
+rewrite -eqC (_ : [set _ in _ | _] = gscc_of x)// in Csccs *.
+by apply/setP => y; rewrite !inE mem_scc /=.
 Qed.
-
-Theorem tarjan_correct : tarjan = gsccs.
-Proof. by rewrite /tarjan; have [->] := tarjan_recP. Qed.
 
 End tarjan.
